{
 "cells": [
  {
   "cell_type": "markdown",
   "metadata": {},
   "source": [
    "<p style=\"page-break-after: always\"></p>\n",
    "\n",
    "# Problem 1\n",
    "Recall that a distortion map $\\phi: E \\rightarrow E$ satisfies that $\\phi(nP) = n\\phi(P)$ for all $P \\in E[l]$.\n",
    "\n",
    "Given $P, aP, bP, cP$, we can pair $P$ with $cP$, $aP$ with $bP$, and compute the modified Weil pairing of each pair:\n",
    "\n",
    "$$\n",
    "\\begin{aligned}\n",
    "\\hat{e}_l(aP, bP) &= e_l(aP, \\phi(bP)) \\\\\n",
    "&= e_l(aP, b\\cdot \\phi(P)) \\\\\n",
    "&= e_l(P, \\phi(P))^{ab} \\\\\n",
    "\\hat{e}_l(P, cP) &= e_l(P, \\phi(cP)) \\\\\n",
    "&= e_l(P, c\\phi(P)) \\\\\n",
    "&= e_l(P, \\phi(P))^c\n",
    "\\end{aligned}\n",
    "$$\n",
    "\n",
    "Divide the first pairing by the second:\n",
    "\n",
    "$$\n",
    "\\frac{\\hat{e}_l(aP, bP)}{\\hat{e}_l(P, cP)} = e_l(P, \\phi(P))^{ab - c}\n",
    "$$\n",
    "\n",
    "Recall that $P$ is a point of finite order $l$, so $(ab)P = cP$ if and only if $ab \\equiv c \\mod l$. On the other hand, because $\\phi$ is a distortion map, $e_l(P, \\phi(P))^{ab - c} = 1$ if and only if $ab - c \\equiv 0 \\mod l$, which is equivalent to $ab \\equiv c \\mod l$. In other words, $e_l(P, \\phi(P))^{ab - c} = 1$ if and only if $(ab)P = cP$.\n",
    "\n",
    "Hence we can solve the ECDDH problem using the distortion map and modified Weil pairing by computing the fraction $\\frac{\\hat{e}_l(aP, bP)}{\\hat{e}_l(P, cP)}$ and checking if it is equal to $1$. This fraction is 1 if and only if $(ab)P = cP$.\n",
    "\n",
    "$$\n",
    "$$\n",
    "$$\n",
    "$$\n",
    "$$\n",
    "$$\n",
    "$$\n",
    "$$\n",
    "$$\n",
    "$$\n",
    "$$\n",
    "$$\n",
    "$$\n",
    "$$\n",
    "$$\n",
    "$$\n",
    "$$\n",
    "$$\n",
    "$$\n",
    "$$\n",
    "$$\n",
    "$$"
   ]
  },
  {
   "cell_type": "markdown",
   "metadata": {},
   "source": [
    "<p style=\"page-break-after: always\"></p>\n",
    "\n",
    "# Problem 2\n",
    "\n",
    "## a)\n",
    "To prove that $\\phi(P) \\in E(\\mathbb{K})$ it suffices to show that $(\\beta x, y)$ satisfies the elliptic curve. \n",
    "\n",
    "For $P = \\mathcal{O}$, this statement is trivial, because $\\phi(\\mathcal{O}) = \\mathcal{O}$ is trivially on the elliptic curve. \n",
    "\n",
    "Now assuming that $P = (x, y) \\neq \\mathcal{O}$, substitute $\\beta x$ for $x$ on the right hand side:\n",
    "\n",
    "$$\n",
    "\\begin{aligned}\n",
    "\\text{R.H.S.} &= (\\beta x)^3 + 1 \\\\\n",
    "&= \\beta^3 x^3 + 1 \\\\\n",
    "&= 1^3 x^3 + 1 \\\\\n",
    "&= x^3 + 1 \\\\\n",
    "&= y^2 = \\text{L.H.S.} \\\\\n",
    "\\end{aligned}\n",
    "$$\n",
    "\n",
    "Thus we've shown that $\\phi(P)$ is also on the curve.\n",
    "\n",
    "## b)\n",
    "We claim that $\\phi(-P) = -\\phi(P)$. This statement trivially true for $P = \\mathcal{O}$ since $-\\mathcal{O} = \\mathcal{O}$. On the other hand, if $P = (x, y) \\neq \\mathcal{O}$, then $\\phi(-P) = \\phi(x, -y) = (\\beta x, -y) = -(\\beta x, y) = - \\phi(P)$.\n",
    "\n",
    "We will prove the addition law, first by discussing a few trivial edge cases, then showing the general case.\n",
    "\n",
    "Trivial case 1: If either of $P_1, P_2$ is $\\mathcal{O}$, then the addition law is trivially held: $\\phi(P_1 + \\mathcal{O}) = \\phi(P_1) = \\phi(P_1) + \\mathcal{O} = \\phi(P_1) + \\phi(\\mathcal{O})$.\n",
    "\n",
    "Trivial case 2: if $P_1 = -P_2$, then $\\phi(P_1 + P_2) = \\phi(\\mathcal{O}) = \\mathcal{O} = \\phi(P_1) - \\phi(P_1) = \\phi(P_1) +\\phi(-P_1) = \\phi(P_1) + \\phi(P_2)$, so the addition law still holds.\n",
    "\n",
    "Now we can assume that neither $P_1, P_2$ is $\\mathcal{0}$ and that $P_1 \\neq -P_2$. Let $P_1 = (x_1, y_1)$, $P_2 = (x_2, y_2)$. Recall the elliptic curve addition formula for $P_3 = (x_3, y_3) = P_1 + P_2$:\n",
    "\n",
    "$$\n",
    "\\begin{cases}\n",
    "x_3 = \\lambda^2 - x_1 - x_2 \\\\\n",
    "y_3 = \\lambda(x_1 - x_3) - y_1\n",
    "\\end{cases}\n",
    "$$\n",
    "\n",
    "Where $\\lambda$ is the slope of the line crossing through the two points, or the tagent line if $P_1 = P_2$. For convenience, we further denote the slope of the line/tagent line running through $\\phi(P_1), \\phi(P_2)$ by $\\lambda_\\phi$, and the denote the point $\\phi(P_1) + \\phi(P_2)$ by $P_3^\\prime = (x_3^\\prime, y_3^\\prime)$\n",
    "\n",
    "If $P_1 \\neq P_2$, then $\\lambda = (y_2 - y_1)(x_2 - x_1)^{-1}$, and $\\lambda_\\phi = (y_2 - y_1)(\\beta x_2 - \\beta x_1)^{-1} = \\lambda\\beta^{-1} = \\lambda\\beta^2$. If $P_1 = P_2$, then $\\lambda = (3x_1^2 + A)(2y_1)^{-1} = (3x_1^2)(2y_1)^{-1}$, and $\\lambda_\\phi = (3(\\beta x)^2 + A)(2y_1)^{-1} = \\beta^2(3x_1^2)(2y_1)^{-1} = \\lambda\\beta^2$. Therefore, **regardless of whether it is a tagent line or a slope**:\n",
    "\n",
    "$$\n",
    "\\lambda_\\phi = \\lambda\\beta^2\n",
    "$$\n",
    "\n",
    "We can now prove the addition law by proving $\\phi(P_3) = P_3^\\prime$ for each coordinate:\n",
    "\n",
    "$$\n",
    "\\begin{aligned}\n",
    "x(P_3^\\prime) &= x(\\phi(P_1) + \\phi(P_2)) \\\\\n",
    "&= \\lambda_\\phi^2 - x(\\phi(P_1)) - x(\\phi(P_2)) \\\\\n",
    "&= (\\lambda\\beta^2)^2 - \\beta x_1 - \\beta x_2 \\\\\n",
    "&= \\lambda^2\\beta^4 - \\beta x_1 - \\beta x_2 \\\\\n",
    "&= \\lambda^2\\beta - \\beta x_1 - \\beta x_2 \\\\\n",
    "&= \\beta(\\lambda - x_1 - x_2) \\\\\n",
    "&= x(\\phi(P_1 + P_2)) \\\\\n",
    "&= x(\\phi(P_3)) \\\\\n",
    "y(P_3^\\prime) &= y(\\phi(P_1) + \\phi(P_2)) \\\\\n",
    "&= \\lambda_\\phi(\\beta x_1 - \\beta x_3) - y_1 \\\\\n",
    "&= \\lambda\\beta^2 \\cdot \\beta(x_1 - x_3) - y_1 \\\\\n",
    "&= \\lambda(x_1 - x_3) - y_1 \\\\\n",
    "&= y(P_3) \\\\\n",
    "&= y(\\phi(P_3))\n",
    "\\end{aligned}\n",
    "$$\n",
    "\n",
    "Thus $\\phi(P_3)$ and $P_3^\\prime$ are coordinate-wise equal.\n"
   ]
  },
  {
   "cell_type": "markdown",
   "metadata": {},
   "source": [
    "<p style=\"page-break-after: always\"></p>\n",
    "\n",
    "# Problem 3\n",
    "\n",
    "## a)\n",
    "Suppose that $x \\in \\mathbb{F}_p$ is a primitive cubic roots, then $x^2$ cannot be $1$ because $x^2 \\equiv x^3 \\equiv 1 \\mod p$ implies $x \\equiv 1 \\mod p$. Thus we know that the (multiplicative) order of $x$ is 3.\n",
    "\n",
    "By Fermat's little theorem we also know that $x^{p-1} \\equiv 1 \\mod p$, which means that $p - 1$ must be a multiple of 3, but we know $p \\equiv 2 \\mod 3$, so $p-1 \\equiv 1 \\mod 3$ could never be a multiple of 3. Therefore, we've arrived at a contradiction, so primitive cubic root cannot exist in $\\mathbb{F}_p$ for $p \\equiv 2 \\mod 3$.\n",
    "\n",
    "To prove that $\\mathbb{F}_{p^2}$ has primitive cube, we'll use the following two facts:\n",
    "\n",
    "1. the multiplicative group $\\mathbb{F}^\\times_{p^2}$ is a finite cyclic group\n",
    "2. if $d$ divides the order of some cyclic group $G$, then there exists a sub-group of order $d$\n",
    "\n",
    "Observe that the multiplicative group $\\mathbb{F}^\\times_{p^2}$ is formed by taking all the non-zero elements, so the order of the multiplicative group is exactly:\n",
    "\n",
    "$$\n",
    "\\vert\\mathbb{F}^\\times_{p^2}\\vert = p^2 - 1\n",
    "$$\n",
    "\n",
    "Because $p \\equiv 2 \\mod 3$, we know 3 divides $p^2 - 1$, which means that there exists cyclic subgroup of $\\mathbb{F}^\\times_{p^2}$ with order 3, and the generator of such cyclic subgroup of order 3 would be a primitive cube root.\n",
    "\n",
    "## b)\n",
    "From problem 2 part (b) we have already proved the addition law $\\phi(P + Q) = \\phi(P) + \\phi(Q)$. From the addition law we can deduce $\\phi(nP) = \\phi(P + (n-1)P) = \\phi(P) + \\phi((n-1)P) = \\ldots = n\\phi(P)$, thus satisfying the first condition of a distortion map.\n",
    "\n",
    "To prove that $e_l(P, \\phi(P))$ is a primitive $l$-th root, we use proposition 6.50 from the textbook, which states that $e_l(P, \\phi(P))$ is a primitive $l$-th root if and only if $P$ is not $\\mathcal{O}$ and $\\phi(P)$ is not a multiple of $P$. Since $P \\in E[l]$ for some $l \\geq 5$, it's trivially true that $P \\neq \\mathcal{O}$. It remains to prove that $\\phi(P)$ is not a multiple of $P$.\n",
    "\n",
    "Suppose that $\\phi(P)$ is a multiple of $P$. Denote the coordinates of $P$ by $(x, y)$ for some $x, y \\in \\mathbb{F}_p$, then the coordinates of any multiples of $P$ must also be in $\\mathbb{F}_p$. However, since we proved in part (a) that $\\beta \\not\\in \\mathbb{F}_p$, $\\phi(P) = (\\beta x, y)$'s coordinates are in $\\mathbb{F}_p$ if and only if $x = 0$, so $P$ must be $(0, \\pm 1)$.\n",
    "\n",
    "Observe the computation of $P + P$:\n",
    "\n",
    "- The tangent line's slope is $\\lambda = (3x^2)(2y)^{-1} = 0$\n",
    "- $x' = \\lambda^2 - x - x = 0$\n",
    "- $y' = \\lambda(x - x_3) - y = \\mp 1$\n",
    "\n",
    "In other words, $P + P = -P$, so $P$ has order 3, which contradicts the fact that $P \\in E[l]$ for prime $l \\geq 5$. Therefore, $\\phi(P)$ is not a multiple of $P$, and $e_l(P, \\phi(P))$ is indeed a primitive $l$-th root."
   ]
  },
  {
   "cell_type": "markdown",
   "metadata": {},
   "source": [
    "<p style=\"page-break-after: always\"></p>\n",
    "\n",
    "# Problem 4\n",
    "First we recall the Boneh-Franklin cryptosystem (and establish some notations):\n",
    "\n",
    "1. $\\mathbb{F}_q, E, l, P, H_1, H_2, B, \\phi, \\hat{e}_l\\leftarrow \\text{PGen}(1^\\lambda)$ where\n",
    "    - $q, l$ are prime numbers\n",
    "    - $E$ is an elliptic curve over the field $\\mathbb{F}_q$\n",
    "    - $P \\in E(\\mathbb{F}_q)[l]$ is a point of finite order $l$\n",
    "    - $H_1: \\{\\text{User IDs}\\} \\rightarrow E[l]$ is a hash function\n",
    "    - $H_2: \\mathbb{F}_q^\\times \\rightarrow \\{0, 1\\}^B$ is another hash function\n",
    "    - $B$ is the bit-length of the message space\n",
    "    - $\\phi$ is a distortion map and $\\hat{e}_l$ is the modified Weil-pairing based on $\\phi$\n",
    "2. $\\text{pk}_\\text{auth}, \\text{sk}_\\text{auth} \\leftarrow \\text{AuthKeyGen}$ generates the authority's key pair, where\n",
    "    - $s \\leftarrow \\mathbb{Z}_l$ is a random integer\n",
    "    - $\\text{sk} \\leftarrow s$ is the authority's secret key\n",
    "    - $\\text{pk} \\leftarrow sP$ is the authority's public key\n",
    "3. $\\text{pk}_\\text{Alice}, \\text{sk}_\\text{Alice} \\leftarrow \\text{UserKeyGen}$ generates the user's key pair, where\n",
    "    - Alice's public key is its user ID\n",
    "    - $P_A \\leftarrow H_1(\\text{Alice's user ID})$\n",
    "    - $\\text{sk}_\\text{Alice} \\leftarrow sP_A$ is Alice's secret key. This secret key is computed by the authority and securely delivered to Alice\n",
    "\n",
    "To encrypt a message $m \\in \\{0, 1\\}^B$, sample a random integer $r \\leftarrow \\{2, 3, \\ldots, q-1\\}$ and compute:\n",
    "\n",
    "$$\n",
    "\\begin{cases}\n",
    "c_1 = rP \\\\\n",
    "c_2 = m \\oplus H_2(\\hat{e}_l(P_A, sP)^r)\n",
    "\\end{cases}\n",
    "$$\n",
    "\n",
    "$c = (c_1, c_2)$ is the encryption.\n",
    "\n",
    "First note that **regardless of the choice of hash function, the Boneh-Franklin cryptosystem is OW-CCA2 insecure**. This is because given a valid ciphertext $c = (c_1, c_2)$, $c' = (c_1, m' \\oplus c_2)$ is also a valid ciphertext. When the adversary receives the challenge ciphertext $c^\\ast = (c_1^\\ast, c_2^\\ast)$, it can generate some random non-zero bit string $m'$ and issue a decryption query on $(c_1^\\ast, m' \\oplus c_2^\\ast)$. The decryption will be $m' \\oplus m^\\ast$, where $m^\\ast$ is the challenge plaintext, and since the adversary knows $m'$, it can recover $m^\\ast$.\n",
    "\n",
    "For the remainder of this discussion, we focus on what happens when $H_1$ returns a multiple of the base point $P$ instead of a truly random point of finite order $l$. However, it is not exactly clear whether $H_1$ returns an opaque multiple $kP$ without revealing or a clear multiple $kP$ that reveals the $k$, so we will discuss the two cases separately:\n",
    "\n",
    "1. $H_1$ returns an opaque multiple $kP$ without giving away $k$\n",
    "2. $H_1$ directly returns $k$\n",
    "\n",
    "Note that these two cases are distinct because recovering $k$ from $P, kP$ is solving the EC discrete log problem, which is conjectured to be hard.\n",
    "\n",
    "## 1)\n",
    "If $H_1$ does not give away the discrete log, then I suspect that Boneh-Franklin's IBE is IND-CPA secure. This is because $c_1$ is independent of the message, while in $c_2$, $H_2$ functions as a pseudorandom one-time pad. Assuming $H_2$ to be collision resistant, the only way to distinguish outputs of $H_2$ is to be able to compute the modified Weil pairing:\n",
    "\n",
    "$$\n",
    "\\hat{e}_l(P_A, sP)^r = \\hat{e}_l(P, P)^{ksr}\n",
    "$$\n",
    "\n",
    "from $kP, sP, rP$, but this is precisely the bilinear Diffie-Hellman problem, which is conjectured to be computationally infeasible.\n",
    "\n",
    "## 2)\n",
    "Now suppose that instead of outputing a random point of finite order $P_a \\leftarrow E[l]$, $H_1$ outputs a random integer $k \\leftarrow \\{1, 2, \\ldots, l-1\\}$, and the authority/encryptor computes Alice's public base point $P_A \\leftarrow kP$. In this scenario, this cryptosystem is **one-way ciphertext-only-attack insecure**, meaning that an adversary can decrypt arbitrary message using only the public keys and the ciphertext.\n",
    "\n",
    "Recall from previous argument, if the adversary can compute $\\hat{e}_l(P, P)^{ksr}$, then it can apply $H_2$ and obtain the mask. The adversary can then use the mask to recover the message:\n",
    "\n",
    "$$\n",
    "m = c_2 \\oplus H_2(\\hat{e}_l(P_A, sP)^r) = c_2 \\oplus H_2(\\hat{e}_l(kP, sP)^r) = c_2 \\oplus H_2(\\hat{e}_l(P, P)^{ksr})\n",
    "$$\n",
    "\n",
    "Indeed if $H_1$ outputs $k$, then the adversary can use $rP$ (which is the first component of the ciphertext and thus public), $sP$ (authority's public key) and $k$ (adversary can obtain $k$ by feeding Alice's user ID into $H_1$) to compute $\\hat{e}_l(P, P)^{ksr}$:\n",
    "\n",
    "$$\n",
    "\\hat{e}_l(rP, sP)^k = \\hat{e}_l(P, P)^{ksr}\n",
    "$$\n",
    "\n",
    "Therefore, the adversary can decrypt arbitrary ciphertext."
   ]
  }
 ],
 "metadata": {
  "kernelspec": {
   "display_name": ".venv",
   "language": "python",
   "name": "python3"
  },
  "language_info": {
   "name": "python",
   "version": "3.10.4"
  }
 },
 "nbformat": 4,
 "nbformat_minor": 2
}
