{
 "cells": [
  {
   "cell_type": "markdown",
   "metadata": {},
   "source": [
    "# Problem 1\n",
    "\n",
    "## a)\n",
    "For each of the prime $p \\in \\{3, 11, 17\\}$, if the integer $a$ is not co-prime with $p$, then $p \\mid a$, and the congruences are trivially true because both sides equal to 0. For the remainder of this argument, for each of the possible prime $p$, we assume $a$ to be co-prime with $p$, which means that Fermat's little theorem holds.\n",
    "\n",
    "For $p = 3$, $a^2 \\equiv 1 \\mod 3$:\n",
    "\n",
    "$$\n",
    "\\begin{aligned}\n",
    "a^{561} &\\equiv a^{2 \\cdot 280 + 1} \\mod 3 \\\\\n",
    "&\\equiv (a^2)^{280} \\cdot a \\mod 3 \\\\\n",
    "&\\equiv 1^{280} \\cdot a \\mod 3 \\\\\n",
    "&\\equiv a \\mod 3\n",
    "\\end{aligned}\n",
    "$$\n",
    "\n",
    "For $p = 11$, we have $a^{10} \\equiv 1 \\mod 11$\n",
    "\n",
    "$$\n",
    "\\begin{aligned}\n",
    "a^{561} &\\equiv a^{10 \\cdot 56 + 1} \\mod 11 \\\\\n",
    "&\\equiv (a^{10})^{56} \\cdot a \\mod 11 \\\\\n",
    "&\\equiv 1^{56} \\cdot a \\mod 11 \\\\\n",
    "&\\equiv a \\mod 11\n",
    "\\end{aligned}\n",
    "$$\n",
    "\n",
    "For $p = 17$, we have $a^{16} \\equiv 1 \\mod 17$:\n",
    "\n",
    "$$\n",
    "\\begin{aligned}\n",
    "a^{561} &\\equiv a^{16 \\cdot 35 + 1} \\mod 17 \\\\\n",
    "&\\equiv (a^{16})^{35} \\cdot a \\mod 17 \\\\\n",
    "&\\equiv 1^{35} \\cdot a \\mod 17 \\\\\n",
    "&\\equiv a \\mod 17\n",
    "\\end{aligned}\n",
    "$$\n",
    "\n",
    "Thus we've shown that the three individual congruences hold for all integers $a$.\n",
    "\n",
    "The fact that the three prime congruences imply the composite congruences is a result of the Chinese remainder theorem. First we take $p = 3$ and $p = 11$ and write out the congruence as Euclidean division:\n",
    "\n",
    "$$\n",
    "a^{561} = m \\cdot 3 + a = n \\cdot 11 + a\n",
    "$$\n",
    "\n",
    "Where $m, n$ are integers. Removing the remainder $a$ we have $m \\cdot 3 = n \\cdot 11$, which implies that $11 \\mid m$. Taking the congruences wiht $p = 3$ and $p = 17$ we can also deduce that $17 \\mid m$. Therefore, $m = 11 \\cdot 17 \\cdot k$ for some other integer $k$, and we can rewrite the Euclidean division above as:\n",
    "\n",
    "$$\n",
    "a^{561} = k \\cdot 11 \\cdot 17 \\cdot 3 + a = k \\cdot 561 + a\n",
    "$$\n",
    "\n",
    "Thus we have $a^{561} \\equiv a \\mod 561$\n",
    "\n",
    "## b)\n",
    "We will prove that the product of two distinct primes cannot be a Carmichael number by showing that **if a Carmichael number is the product of two primes, then the two primes must be equal**.\n",
    "\n",
    "Let $n = p \\cdot q$ be a Carmichael number that is the product of two primes $p, q$. By the definition of a Carmichael number we know that $a^{p \\cdot q} \\equiv a \\mod n$ for all integers a.\n",
    "\n",
    "By Chinese remainder theorem, we know that $a^{pq} \\equiv a \\mod p$ for all integers $a$. This means that this congruence hold for the primitive root(s) of $p$, as well. From assignment 1 we know that because $p$ is prime, at least one primitive root exists, and we will denote it by $g$. By the definition of primitive roots we know that the order of $g$ is $p-1$.\n",
    "\n",
    "By Fermat's little theorem we know that $g^p \\equiv g \\mod p$, so $g^{pq} \\equiv g^q \\equiv g \\mod p$. Because $g$ is a primitive root and thus has a multiplicative inverse, we can multiply $g^{-1}$ on the congruence to get $g^{q-1} \\equiv 1 \\mod p$. From assignment 1 we know that the order of $g$ must thus divide $q-1$, which means that $p - 1 \\mid q - 1$.\n",
    "\n",
    "Swapping $p, q$ in the two paragraphs above, we can also deduce that $q - 1 \\mid p - 1$. This necessarily means that $p - 1 = q - 1$, so $p = q$.\n",
    "\n",
    "## c)\n",
    "When $n$ is even, $-1 \\equiv n - 1 \\mod n$ is always a Fermat witness because $-1$ raised to an even power is always $1$"
   ]
  },
  {
   "cell_type": "markdown",
   "metadata": {
    "jp-MarkdownHeadingCollapsed": true
   },
   "source": [
    "<p style=\"page-break-after: always\"></p>\n",
    "\n",
    "# Problem 2\n",
    "**Credits: proof derived from K. Ireland, M. Rosen, *A Classical Introduction to Modern Number Theory***\n",
    "\n",
    "We begin by deriving a number of lemmas before proving the actual results.\n",
    "\n",
    "**(Lemma 1)** if $a, b$ are odd integers, then \n",
    "\n",
    "$$\n",
    "\\frac{a-1}{2} + \\frac{b-1}{2} \\equiv \\frac{ab-1}{2} \\mod 2\n",
    "$$\n",
    "\n",
    "**Proof**: First observe that $a-1, b-1$ are both even, so $(a-1)(b-1) \\equiv 0 \\mod 4$. Rearranging this congruence we have $ab -1 \\equiv (a - 1) + (b - 1) \\mod 4$, which implies that $ab - 1 = 4k + (a - 1) + (b-1)$ for some integer $k$. Divide both sides by 2 we have\n",
    "\n",
    "$$\n",
    "\\frac{ab-1}{2} = 2k + \\frac{a-1}{2} + \\frac{b-1}{2}\n",
    "$$\n",
    "\n",
    "This proves Lemma 1.\n",
    "\n",
    "**(Lemma 2)** if $p_1, p_2, \\ldots, p_t$ are odd integers, then\n",
    "\n",
    "$$\n",
    "\\sum_{i=1}^t \\frac{p_i - 1}{2} \\equiv \\frac{(\\prod_{i=1}^t p_i) - 1}{2} \\mod 2\n",
    "$$\n",
    "\n",
    "**Proof**: we will prove by induction. The base case where $t = 1$ is trivial. Now suppose the congruence to hold for $t = n$, then\n",
    "\n",
    "$$\n",
    "\\begin{aligned}\n",
    "\\sum_{i=1}^{n+1} \\frac{p_i - 1}{2} &= \\sum_{i=1}^{n} \\frac{p_i - 1}{2} + \\frac{p_{n+1}-1}{2} \\\\\n",
    "&\\equiv \\frac{(\\prod_{i=1}^n p_i) - 1}{2} + \\frac{p_{n+1}-1}{2} \\mod 2\n",
    "\\end{aligned}\n",
    "$$\n",
    "\n",
    "Because the product of odd integers is an odd integer, we can apply Lemma 1 to RHS:\n",
    "\n",
    "$$\n",
    "\\frac{(\\prod_{i=1}^n p_i) - 1}{2} + \\frac{p_{n+1}-1}{2} = \\frac{(\\prod_{i=1}^{n+1} p_i) - 1}{2}\n",
    "$$\n",
    "\n",
    "Thus we have proved the inductive case.\n",
    "\n",
    "**(Lemma 3)** if $a, b$ are odd integers, then\n",
    "\n",
    "$$\n",
    "\\frac{a^2b^2 - 1}{8} \\equiv \\frac{a^2 - 1}{8} + \\frac{b^2 - 1}{8} \\mod 2\n",
    "$$\n",
    "\n",
    "**Proof:** First observe that for odd integer $a$, $a^2 - 1$ is divisible by 4. This is because $a^2 - 1 = (a+1)(a-1)$, where $a+1, a-1$ are both even, and the product of two even numbers is guaranteed to be divisible by 4. Therefore we know that $a^2 - 1 \\equiv b^2 - 1 \\equiv 0 \\mod 4$, which means that $a^2 - 1 = 4k, b^2 - 1 = 4l$ for some integers $k, l$. Multiply the two equations, we get $(a^2 - 1)(b^2 - 1) = 16kl$, therefore:\n",
    "\n",
    "$$\n",
    "(a^2 - 1)(b^2 - 1) \\equiv 0 \\mod 16\n",
    "$$\n",
    "\n",
    "Rearranging the congruence above:\n",
    "\n",
    "$$\n",
    "a^2b^2 - 1 \\equiv (a^2 - 1) + (b^2 - 1) \\mod 16\n",
    "$$\n",
    "\n",
    "Which implies that for some integer $k$:\n",
    "\n",
    "$$\n",
    "a^2b^2 - 1 = 16k + (a^2 - 1) + (b^2 - 1)\n",
    "$$\n",
    "\n",
    "Divide both sides by 8, we get:\n",
    "\n",
    "$$\n",
    "\\frac{a^2b^2 - 1}{8} = 2k + \\frac{a^2 - 1}{8} + \\frac{b^2-1}{8}\n",
    "$$\n",
    "\n",
    "This proves the lemma\n",
    "\n",
    "**Lemma 4**: let $p_1, p_2, \\ldots, p_t$ be odd integers, then\n",
    "\n",
    "$$\n",
    "\\sum_{i=1}^{t}\\frac{p_i^2 - 1}{8} \\equiv \\frac{(\\prod_{i=1}^{t}p_i^2) - 1}{8} \\mod 2\n",
    "$$\n",
    "\n",
    "**Proof:** again we will prove by induction, and again the base case $t = 1$ is trivial. Now suppose the congruence hold for $t = n$, then \n",
    "\n",
    "$$\n",
    "\\begin{aligned}\n",
    "\\sum_{i=1}^{n+1}\\frac{p_i^2 - 1}{8} &\\equiv \\sum_{i=1}^{n}\\frac{p_i^2 - 1}{8} + \\frac{p_{n+1}^2 - 1}{8} \\mod 2 \\\\\n",
    "&\\equiv \\frac{(\\prod_{i=1}^{n}p_i^2) - 1}{8} + \\frac{p_{n+1}^2 - 1}{8} \\mod 2 \\\\\n",
    "&\\equiv \\frac{(\\prod_{i=1}^{n}p_i)^2 - 1}{8} + \\frac{p_{n+1}^2 - 1}{8} \\mod 2\n",
    "\\end{aligned}\n",
    "$$\n",
    "\n",
    "Apply Lemma 3 to RHS:\n",
    "\n",
    "$$\n",
    "\\frac{(\\prod_{i=1}^{n}p_i)^2 - 1}{8} + \\frac{p_{n+1}^2 - 1}{8} \\equiv \\frac{(\\prod_{i=1}^{n+1}p_i^2) - 1}{8} \\mod 2\n",
    "$$\n",
    "\n",
    "Thus we've proved Lemma 4.\n",
    "\n",
    "Last but not least we claim a trivial result: $(-1)^a = (-1)^b$ if and only if $a \\equiv b \\mod 2$. For the remainder of the writeup, these four lemmas and the trivial result will be directly used without explicit declaration.\n",
    "\n",
    "## a)\n",
    "$$\n",
    "\\begin{aligned}\n",
    "\\bigg(\\frac{-1}{n}\\bigg) &= \\bigg(\\frac{-1}{p_1}\\bigg)\n",
    "\\bigg(\\frac{-1}{p_2}\\bigg)\n",
    "\\ldots\n",
    "\\bigg(\\frac{-1}{p_t}\\bigg) \\\\\n",
    "&= \\prod_{i=1}^t (-1)^\\frac{p_i - 1}{2} \\\\\n",
    "&= (-1)^{\\sum_{i=1}^t\\frac{p_i - 1}{2}} \\\\\n",
    "&= (-1)^{\\frac{(\\prod_{i=1}^t p_i) - 1}{2}} \\\\\n",
    "&= (-1)^\\frac{n-1}{2}\n",
    "\\end{aligned}\n",
    "$$\n",
    "\n",
    "## b)\n",
    "$$\n",
    "\\begin{aligned}\n",
    "\\bigg(\\frac{2}{n}\\bigg) &= \\bigg(\\frac{2}{p_1}\\bigg)\n",
    "\\bigg(\\frac{2}{p_2}\\bigg)\n",
    "\\ldots\n",
    "\\bigg(\\frac{2}{p_t}\\bigg) \\\\ \n",
    "&= \\prod_{i=1}^t (-1)^\\frac{p_i^2 - 1}{8} \\\\\n",
    "&= (-1)^{\\sum_{i=1}^t\\frac{p_i^2 - 1}{8}} \\\\\n",
    "&= (-1)^{\\frac{(\\prod_{i=1}^{t}p_i^2) - 1}{8}} \\\\\n",
    "&= (-1)^{\\frac{(\\prod_{i=1}^{t}p_i)^2 - 1}{8}} \\\\\n",
    "&= (-1)^{\\frac{n^2 - 1}{8}} \\\\\n",
    "\\end{aligned}\n",
    "$$\n",
    "\n",
    "## c)\n",
    "First we claim a trivial result:\n",
    "\n",
    "Let $p$ be a prime number, then the Legendre symbol of a product is the product of Legendre symbol $(\\frac{ab}{p}) = (\\frac{a}{p})(\\frac{b}{p})$. For $a, b$ that are co-prime with $p$, this can be proved using Euler's criterion: $(\\frac{a}{p})(\\frac{b}{p}) \\equiv a^\\frac{p-1}{2}b^\\frac{p-1}{2} \\equiv (ab)^\\frac{p-1}{2} = (\\frac{ab}{p})$; if any of $a, b$ is not co-prime with $p$, then both sides are trivially 0\n",
    "\n",
    "Now suppose $m, n$ has prime factorization:\n",
    "\n",
    "$$\n",
    "m = p_1p_2\\ldots p_t \\\\\n",
    "n = q_1q_2 \\ldots q_s\n",
    "$$\n",
    "\n",
    "Then\n",
    "\n",
    "$$\n",
    "\\begin{aligned}\n",
    "\\bigg(\\frac{m}{n}\\bigg) &= \\bigg(\\frac{\\prod_{i=1}^tp_i}{\\prod_{j=1}^s q_j}\\bigg) \\\\\n",
    "&= \\prod_{i=1}^t\\prod_{j=1}^s\\bigg(\\frac{p_i}{q_j}\\bigg)\n",
    "\\end{aligned}\n",
    "$$\n",
    "\n",
    "Similarly we have\n",
    "\n",
    "$$\n",
    "\\begin{aligned}\n",
    "\\bigg(\\frac{n}{m}\\bigg) &= \\bigg(\\frac{\\prod_{j=1}^s q_j}{\\prod_{i=1}^tp_i}\\bigg) \\\\\n",
    "&= \\prod_{i=1}^t\\prod_{j=1}^s\\bigg(\\frac{q_j}{p_i}\\bigg)\n",
    "\\end{aligned}\n",
    "$$\n",
    "\n",
    "Multiply the two equations:\n",
    "\n",
    "$$\n",
    "\\begin{aligned}\n",
    "\\bigg(\\frac{m}{n}\\bigg)\\bigg(\\frac{n}{m}\\bigg) &= \\prod_{i=1}^t\\prod_{j=1}^s\\bigg(\\frac{p_i}{q_j}\\bigg) \\cdot \\prod_{i=1}^t\\prod_{j=1}^s\\bigg(\\frac{q_j}{p_i}\\bigg) \\\\\n",
    "&= \\prod_{i=1}^t\\prod_{j=1}^s\\bigg(\\frac{p_i}{q_j}\\bigg)\\bigg(\\frac{q_j}{p_i}\n",
    "\\bigg) \\\\\n",
    "&= \\prod_{i=1}^t\\prod_{j=1}^s(-1)^\\frac{(p_i - 1)(q_j - 1)}{4} \\\\\n",
    "&= (-1)^{\\sum_{i=1}^t\\sum_{j=1}^s\\frac{(p_i - 1)(q_j - 1)}{4}}\n",
    "\\end{aligned}\n",
    "$$\n",
    "\n",
    "Observe the exponent:\n",
    "\n",
    "$$\n",
    "\\begin{aligned}\n",
    "\\sum_{i=1}^t\\sum_{j=1}^s\\frac{(p_i - 1)(q_j - 1)}{4} &= \\sum_{i=1}^t (\\frac{p_i - 1}{2} \\sum_{j=1}^s\\frac{q_j - 1}{2}) \\\\ \n",
    "&\\equiv \\sum_{i=1}^t(\\frac{p_i-1}{2} \\cdot \\frac{q_1q_2 \\ldots q_s - 1}{2}) \\mod 2 \\\\\n",
    "&\\equiv \\sum_{i=1}^t(\\frac{p_i-1}{2} \\cdot \\frac{n - 1}{2}) \\mod 2 \\\\\n",
    "&\\equiv \\frac{n - 1}{2} \\sum_{i=1}^t(\\frac{p_i-1}{2}) \\mod 2 \\\\\n",
    "&\\equiv \\frac{n - 1}{2} \\frac{p_1p_2 \\ldots p_t - 1}{2} \\mod 2 \\\\\n",
    "&\\equiv \\frac{n - 1}{2} \\frac{m - 1}{2} \\mod 2 \\\\\n",
    "&\\equiv \\frac{(m-1)(n-1)}{4} \\mod 2\n",
    "\\end{aligned}\n",
    "$$\n",
    "\n",
    "Plugging this into the RHS of the previous equation:\n",
    "\n",
    "$$\n",
    "\\bigg(\\frac{m}{n}\\bigg)\\bigg(\\frac{n}{m}\\bigg) = (-1)^{\\frac{(m-1)(n-1)}{4}}\n",
    "$$"
   ]
  }
 ],
 "metadata": {
  "kernelspec": {
   "display_name": "Python 3 (ipykernel)",
   "language": "python",
   "name": "python3"
  },
  "language_info": {
   "codemirror_mode": {
    "name": "ipython",
    "version": 3
   },
   "file_extension": ".py",
   "mimetype": "text/x-python",
   "name": "python",
   "nbconvert_exporter": "python",
   "pygments_lexer": "ipython3",
   "version": "3.10.4"
  }
 },
 "nbformat": 4,
 "nbformat_minor": 4
}
